Weidenbach_Book/IsaSAT/IsaSAT_LLVM.thy
@@ -457,15 +457,13 @@ definition model_bounded_assn where
    {((b, m), (b', m')). b=b' \<and> (b \<longrightarrow> (m,m') \<in> model_stat_rel)}\<close>
 
 definition clauses_l_assn where
-  \<open>clauses_l_assn = hr_comp (IICF_Array_of_Array_List.aal_assn
-                                    unat_lit_assn)
-                                  (list_mset_rel O
-                                   \<langle>list_mset_rel\<rangle>IsaSAT_Initialisation.mset_rel)\<close>
+  \<open>clauses_l_assn = hr_comp (IICF_Array_of_Array_List.aal_assn unat_lit_assn)
+    (list_mset_rel O \<langle>list_mset_rel\<rangle>IsaSAT_Initialisation.mset_rel)\<close>
 
 theorem IsaSAT_full_correctness:
   \<open>(uncurry IsaSAT_code, uncurry (\<lambda>_. model_if_satisfiable_bounded))
      \<in> [\<lambda>(_, a). Multiset.Ball a distinct_mset \<and>
-      (\<forall>C\<in>#a.  \<forall>L\<in>#C. nat_of_lit L  \<le> uint32_max)]\<^sub>a opts_assn\<^sup>d *\<^sub>a clauses_l_assn\<^sup>k \<rightarrow> model_bounded_assn\<close>
+      (\<forall>C\<in>#a. \<forall>L\<in>#C. nat_of_lit L \<le> uint32_max)]\<^sub>a opts_assn\<^sup>d *\<^sub>a clauses_l_assn\<^sup>k \<rightarrow> model_bounded_assn\<close>
   using IsaSAT_code.refine[FCOMP IsaSAT_bounded_heur_model_if_sat'[unfolded convert_fref]]
   unfolding model_bounded_assn_def clauses_l_assn_def
   apply auto
